chore: utype

RISCV/Instructions.lean
@@ -10,3 +10,18 @@ namespace RV64I
 -/
 def addiw (imm : BitVec 12) (rs1_val : BitVec 64) : BitVec 64 :=
   BitVec.signExtend 64 (BitVec.setWidth 32 (BitVec.add (BitVec.signExtend 64 imm) rs1_val))
+
+/--
+  Build 32-bit constants and uses the U-type format. LUI places the U-immediate value in the top 20
+  bits of the destination register rd, filling in the lowest 12 bits with zeros.
+-/
+def lui (imm : BitVec 20) (_ : BitVec 64) : BitVec 64 :=
+     BitVec.signExtend 64 (imm ++ (0x000 : (BitVec 12)))
+
+/--
+  Build pc-relative addresses and uses the U-type format. AUIPC forms a 32-bit offset from the
+  20-bit U-immediate, filling in the lowest 12 bits with zeros, adds this offset to the pc,
+  then places the result in register rd.
+-/
+def auipc (imm : BitVec 20) (pc : BitVec 64)  : BitVec 64 :=
+    BitVec.add (BitVec.signExtend 64 (BitVec.append imm (0x000 : (BitVec 12)))) pc
