RISCV/SailPure.lean
@@ -11,3 +11,9 @@ namespace SailRV64I
 def addiw (imm : BitVec 12) (rs1_val : BitVec 64) : BitVec 64 :=
   let result :=  rs1_val + (sign_extend (m := ((2 ^i 3) *i 8)) imm)
   (sign_extend (m := ((2 ^i 3) *i 8)) (Sail.BitVec.extractLsb result 31 0))
+
+def utype (imm : (BitVec 20)) (pc : (BitVec 64)) (op : uop)  : BitVec 64 :=
+  let off := (sign_extend (m := ((2 ^i 3) *i 8)) (imm ++ (0x000 : (BitVec 12))))
+  match op with
+  | uop.LUI => off
+  | uop.AUIPC => BitVec.add pc off
