RISCV/Skeleton.lean
@@ -31,9 +31,8 @@ def skeleton_unary (rs1 : regidx) (rd : regidx) (execute_func : BitVec 64 → Bi
 /-- Given an operation `op` with one immediate argument `imm` and a destination register `rd`,
   read the `pc` value and write the result of `op` to the destination register.
 -/
-def skeleton_UTYPE  (imm : BitVec 20) (rd : regidx) (op : uop)
-    (execute_func : BitVec 20 → BitVec 64 → uop → BitVec 64) : SailM ExecutionResult := do
-  let pc ← get_arch_pc ()
+def skeleton_utype  (imm : BitVec 20) (rd : regidx) (op : uop) (execute_func : BitVec 20 → BitVec 64 → uop → BitVec 64) : SailM ExecutionResult := do
+  let pc ← get_arch_pc () -- states that I modelled this model like this bc its more uniform and neat but made the proof more compilcated
   let result := execute_func imm pc op
   wX_bits rd result
   pure RETIRE_SUCCESS
@@ -41,9 +40,18 @@ def skeleton_UTYPE  (imm : BitVec 20) (rd : regidx) (op : uop)
 /-- Given a function `execute_func` with one immediate argument `imm` and a destination register `rd`,
   read the `pc` value and write the result of `execute_func` to the destination register.
 -/
-def skeleton_UTYPE_AUIPC  (imm : BitVec 20) (rd : regidx)
+def skeleton_utype_auipc  (imm : BitVec 20) (rd : regidx)
     (execute_func : BitVec 20 → BitVec 64 → BitVec 64) : SailM ExecutionResult := do
   let pc ← get_arch_pc ();
   let result := execute_func imm pc
+  wX_bits rd result
+  pure RETIRE_SUCCESS
+
+/-- Given a function `execute_func` with one immediate argument `imm` and a destination register `rd`,
+  write the result of `execute_func` to the destination register.
+-/
+def skeleton_utype_lui  (imm : BitVec 20) (rd : regidx)
+    (execute_func : BitVec 20 → BitVec 64 → BitVec 64) : SailM ExecutionResult := do
+  let result := execute_func imm 0#64
   wX_bits rd result
   pure RETIRE_SUCCESS
