RISCV/SailPureToInstructions.lean
@@ -15,3 +15,18 @@ theorem add_eq (imm : BitVec 12) (rs1_val : BitVec 64) :
   rw [BitVec.extractLsb, BitVec.setWidth_eq_extractLsb' (by omega)]
   unfold instHPowInt_leanRV64D
   bv_decide
+
+theorem lui_eq (imm : BitVec 20) (pc : BitVec 64) :
+    SailRV64I.utype imm pc (uop.LUI) = RV64I.lui imm pc := by
+  simp only [SailRV64I.utype, LeanRV64D.Functions.sign_extend, Sail.BitVec.signExtend,
+    BitVec.signExtend, Nat.reduceAdd, BitVec.ofNat_eq_ofNat, lui]
+  unfold instHPowInt_leanRV64D
+  bv_decide
+
+theorem auipc_eq (imm : BitVec 20) (pc : BitVec 64) :
+    SailRV64I.utype imm pc (uop.AUIPC)
+    = RV64I.auipc imm pc:= by
+  simp only [SailRV64I.utype, LeanRV64D.Functions.sign_extend, Sail.BitVec.signExtend,
+    Nat.reduceAdd, BitVec.ofNat_eq_ofNat, BitVec.add_eq, auipc, BitVec.append_eq]
+  unfold instHPowInt_leanRV64D
+  bv_decide
