RISCV/SailToRV64.lean
@@ -10,3 +10,29 @@ open LeanRV64D.Functions
 theorem add_eq (imm : BitVec 12) (rs1 : regidx) (rd : regidx) :
     execute_ADDIW  imm rs1 rd = skeleton_unary rs1 rd (SailRV64I.addiw imm) := by
   simp [execute_ADDIW, skeleton_unary, SailRV64I.addiw]
+
+theorem utype_eq_lui (imm : BitVec 20) (rd : regidx):
+    execute_UTYPE imm rd (uop.LUI) = skeleton_utype_lui imm rd
+    (fun imm' pc => SailRV64I.utype imm' pc uop.LUI) := by
+  simp only [execute_UTYPE, sign_extend, Sail.BitVec.signExtend, Nat.reduceAdd,
+    BitVec.ofNat_eq_ofNat, bind_pure_comp, pure_bind, skeleton_utype_lui, imp_self, implies_true,
+    map_inj_right_of_nonempty]
+  rfl
+
+theorem utype_eq_auipc (imm : (BitVec 20)) (rd : regidx):
+    execute_UTYPE imm rd (uop.AUIPC) = skeleton_utype_auipc imm rd
+    (fun imm' pc => SailRV64I.utype imm' pc uop.AUIPC) := by
+  simp [execute_UTYPE, skeleton_utype_auipc, SailRV64I.utype]
+
+theorem utype_eq (imm : (BitVec 20)) (rd : regidx) (op : uop) (h_pc : s.regs.get? Register.PC = some valt):
+    execute_UTYPE imm rd op s = skeleton_utype imm rd op SailRV64I.utype s := by
+  simp [execute_UTYPE, skeleton_utype, SailRV64I.utype]
+  cases op
+  · simp only [pure_bind]
+    simp only [EStateM.instMonad, EStateM.map, Monad.toBind, get_arch_pc, PreSail.readReg, get,
+      getThe, MonadStateOf.get, EStateM.bind, EStateM.get]
+    rcases hs : s.regs.get? Register.PC
+    · simp [hs] at h_pc
+    · simp only
+      rfl
+  · simp
